feat: New definitions for the memory model (#74)
For freedom in experimenting with definitions, we define our own version
of `read_mem` and `write_mem` called `read_mem'` and `write_mem`'. These
operate directly on the memory, rather than the `ArmState`. We prove
their equivalence to the existing definitions (`read_mem_eq_read_mem'`,
`write_mem_eq_write_mem'`).

Furthermore, we define equivalences to `BitVec.extractLsByte` to ease
reasoning about byte-level manipulation. As an easy corollary, we get
`getLsb` theorems on these in order to allow `omega` based reasoning
about bit-level values of memory.

We then build lemmas that allow simplification of the proof state given
the new `mem_subset'` and `mem_separate'` assumptions. In total, this
gives us automation to simplify theorems about memory
(non)-interference.

### Testing:

What tests have been run? Did `make all` succeed for your changes? Was
conformance testing successful on an Aarch64 machine?

- `make all` succeeded.
- Conformance testing was not run, since the definitions have not
changed.


### License:

By submitting this pull request, I confirm that my contribution is
made under the terms of the Apache 2.0 license.

---------

Co-authored-by: Alex Keizer <alex@keizer.dev>
Co-authored-by: Shilpi Goel <shigoel@gmail.com>

Arm/State.lean
@@ -118,6 +118,12 @@ deriving DecidableEq, Repr
 def PState.zero : PState :=
   { n := 0#1, z := 0#1, c := 0#1, v := 0#1 }
 
+/--
+Memory: maps 64-bit addresses to bytes.
+We use an abbreivation to write definitions that are about memory as `*`.
+-/
+abbrev Memory := Store (BitVec 64) (BitVec 8)
+
 @[ext]
 structure ArmState where
   /-- General-purpose registers: register 31 is the stack pointer. -/
@@ -129,7 +135,7 @@ structure ArmState where
   /-- PState -/
   private pstate     : PState
   /-- Memory: maps 64-bit addresses to bytes -/
-  private mem        : Store (BitVec 64) (BitVec 8)
+  private mem        : Memory
   /--
   Program: maps 64-bit addresses to 32-bit instructions.
   Note that we have the following assumption baked into our machine model:
@@ -660,5 +666,338 @@ theorem write_mem_of_write_mem_shadow :
 theorem write_mem_irrelevant :
   write_mem addr (read_mem addr s) s = s := by
   simp [read_mem, write_mem, store_write_irrelevant]
+
+end Memory
+
+
+/-!
+# New definitions for the memory model
+
+For freedom in experimenting with definitions,
+we define our own version of `read_mem` and `write_mem`,
+called `Memory.read` and `Memory.write`.
+These operate directly on the memory, rather than the `ArmState`.
+We prove their equivalence to the existing definitions
+(`ArmState.read_mem_eq_mem_read`, `ArmState.write_mem_eq_mem_write`).
+
+Furthermore, we define equivalences to `BitVec.extractLsByte`
+to ease reasoning about byte-level manipulation.
+As an easy corollary, we get `getLsb` theorems on these to allow
+`omega` based reasoning about bit-level values of memory.
+-/
+
+/--
+A variant of `read_mem` that directly talks about writes to memory, instead of over the entire `ArmState`
+-/
+def Memory.read (addr : BitVec 64) (m : Memory) : BitVec 8 :=
+  read_store addr m
+
+theorem ArmState.read_mem_eq_mem_read : read_mem addr s = s.mem.read addr := rfl
+
+/--
+A variant of `write_mem` that directly talks about writes to memory, instead of over the entire `ArmState`
+-/
+def Memory.write (addr : BitVec 64) (val : BitVec 8) (m : Memory) : Memory :=
+  write_store addr val m
+
+theorem ArmState.write_mem_eq_mem_write :  (write_mem addr val s).mem = s.mem.write addr val := rfl
+
+namespace Memory
+
+theorem getLsb_read (mem : Memory) : (mem.read addr).getLsb i = (mem addr).getLsb i := rfl
+
+def read_bytes (n : Nat) (addr : BitVec 64) (m : Memory) : BitVec (n * 8) :=
+  match n with
+  | 0 => 0#0
+  | n' + 1 =>
+    let byte := m.read addr
+    let rest := m.read_bytes n' (addr + 1#64)
+    have h : n' * 8 + 8 = (n' + 1) * 8 := by simp_arith
+    BitVec.cast h (rest ++ byte)
+
+theorem State.read_mem_bytes_eq_mem_read_bytes (s : ArmState) :
+    read_mem_bytes n addr s = s.mem.read_bytes n addr := by
+  induction n generalizing addr s
+  case zero => simp [read_mem_bytes, read_bytes]
+  case succ n' ih =>
+    simp [read_mem_bytes, read_bytes, ArmState.read_mem_eq_mem_read, ih]
+
+@[memory_rules]
+theorem read_bytes_zero_eq (m : Memory) : m.read_bytes 0 addr = 0#0 :=
+  rfl
+
+theorem read_bytes_succ_eq (m : Memory) :
+  m.read_bytes (n' + 1) addr = (m.read_bytes n' (addr + 1) ++ m.read addr).cast (by omega) := rfl
+
+theorem getLsb_read_bytes {n i : Nat} {addr : BitVec 64} {m : Memory} (hn : n ≤ 2^64) :
+    (m.read_bytes n addr).getLsb i =
+    (decide (i < n * 8) && (m (addr + BitVec.ofNat 64 (i / 8))).getLsb (i % 8)) := by
+  induction n generalizing i addr m
+  case zero =>
+    simp only [Nat.reduceMul, Nat.zero_le, BitVec.getLsb_ge, Nat.zero_mul, Nat.not_lt_zero,
+      decide_False, Bool.false_and]
+  case succ n' ih =>
+    simp only [read_bytes_succ_eq, BitVec.ofNat_eq_ofNat,
+      BitVec.getLsb_cast, BitVec.getLsb_append, memory_rules,
+      getLsb_read]
+    rw [Nat.succ_mul]
+    by_cases h₁ : (i < 8)
+    · simp only [h₁, decide_True, cond_true, show i < n' * 8 + 8 by omega, Bool.true_and]
+      have hdiv : i / 8 = 0 :=  Nat.div_eq_of_lt h₁
+      rw [hdiv]
+      simp only [BitVec.add_zero]
+      have hmod : i % 8 = i := Nat.mod_eq_of_lt h₁
+      simp [hmod]
+    · simp only [h₁, decide_False, cond_false]
+      rw [ih]
+      by_cases h₂ : i - 8 < n' * 8
+      · simp only [h₂, decide_True, Bool.true_and, show (i < n' * 8 + 8) by omega]
+        have hi' : ∃ i', i = i' + 8 := by
+          apply Classical.byContradiction
+          intros h
+          simp only [not_exists] at h
+          specialize h (i - 8)
+          omega
+        obtain ⟨i', hi'⟩ := hi'
+        subst hi'
+        simp only [Nat.add_sub_cancel, Nat.zero_lt_succ, Nat.add_div_right, Nat.add_mod_right]
+        congr 2
+        rw [BitVec.add_assoc]
+        congr
+        rw [BitVec.add_def]
+        congr 1
+        simp only [BitVec.toNat_ofNat, Nat.reducePow, Nat.reduceMod]
+        rw [Nat.mod_eq_of_lt]
+        · omega
+        · omega
+      · simp only [h₂, decide_False, Bool.false_and, Bool.false_eq, Bool.and_eq_false_imp,
+          decide_eq_true_eq]
+        intros h₃
+        omega
+      · omega
+
+
+/--
+This is a low level theorem.
+Prefer using theorems from `Arm.Separate` that provide higher level theorems
+in terms of memory (non)-interference.
+-/
+theorem write_of_eq {m : Memory} (hix : ix = addr) : m.write addr val ix = val := by
+  simp only [write]
+  subst ix
+  apply store_read_over_write_same
+
+@[memory_rules]
+theorem write_of_eq' {m : Memory} : m.write ix val ix = val := write_of_eq rfl
+
+/--
+This is a low level theorem.
+Prefer using theorems from `Arm.Separate` that provide higher level theorems
+in terms of memory (non)-interference.
+-/
+theorem write_of_neq {m : Memory} (hix : ix ≠ addr) : m.write addr val ix = m ix := by
+  simp only [write]
+  apply store_read_over_write_different
+  assumption
+
+def write_bytes (n : Nat) (addr : BitVec 64)
+    (val : BitVec (n * 8)) (m : Memory) : Memory :=
+  match n with
+  | 0 => m
+  | n' + 1 =>
+    let byte := BitVec.extractLsb 7 0 val
+    let m := m.write addr byte
+    let val_rest := BitVec.zeroExtend (n' * 8) (val >>> 8)
+    m.write_bytes n' (addr + 1#64) val_rest
+
+/-- Writing zero bytes does not change memory. -/
+@[memory_rules]
+theorem write_bytes_zero {m : Memory} : m.write_bytes 0 addr val = m := rfl
+
+@[memory_rules]
+theorem write_mem_bytes_eq_mem_write_bytes (s : ArmState) :
+    write_mem_bytes n addr val s =
+    { s with mem := s.mem.write_bytes n addr val } := by
+  induction n generalizing addr s
+  case zero => simp [write_mem_bytes, write_bytes_zero]
+  case succ n' ih =>
+    simp [write_mem_bytes, ArmState.read_mem_eq_mem_read, ih,
+      write_mem, write_bytes]
+    rfl
+
+/--
+Writing (n + 1) bytes can be described as writing `n` bytes
+and then recursing to write the rest.
+-/
+theorem write_bytes_succ {mem : Memory} :
+    mem.write_bytes (n + 1) addr val =
+    let byte := BitVec.extractLsb 7 0 val
+    let mem := mem.write addr byte
+    let val_rest := BitVec.zeroExtend (n * 8) (val >>> 8)
+    mem.write_bytes n (addr + 1#64) val_rest := rfl
+
+theorem write_bytes_eq_of_le  {mem : Memory} {ix base : BitVec 64}
+    (hix : ix.toNat < base.toNat) (hnowrap : base.toNat + n ≤ 2^64) :
+    mem.write_bytes n base data ix = mem ix := by
+  induction n generalizing base mem ix
+  case zero => simp only [write_bytes]
+  case succ n ih =>
+    simp only [write_bytes]
+    rcases n with rfl | n
+    · rw [write_bytes_zero]
+      apply write_of_neq (BitVec.neq_of_lt hix)
+    · rw [ih]
+      · apply write_of_neq (BitVec.neq_of_lt hix)
+      · rw [BitVec.toNat_add_eq_toNat_add_toNat]
+        · omega
+        · simp only [BitVec.toNat_ofNat, Nat.reducePow, Nat.reduceMod]; omega
+      · rw [BitVec.toNat_add_eq_toNat_add_toNat]
+        · simp only [BitVec.toNat_ofNat, Nat.reducePow, Nat.reduceMod]; omega
+        · simp only [BitVec.toNat_ofNat, Nat.reducePow, Nat.reduceMod]; omega
+theorem write_bytes_eq_of_ge {mem : Memory} {ix base : BitVec 64}
+    (hix : ix.toNat ≥ base.toNat + n)
+    (hnowrap : base.toNat + n ≤ 2^64) :
+    mem.write_bytes n base data ix = mem ix := by
+  induction n generalizing base mem ix
+  case zero => simp [write_bytes]
+  case succ n ih =>
+    simp only [write_bytes]
+    rw [ih]
+    · have hix : ix.toNat > base.toNat := by omega
+      obtain hix : ix.toNat ≠ base.toNat := by omega
+      apply write_of_neq (by apply BitVec.neq_of_toNat_neq hix)
+    · rw [BitVec.toNat_add_eq_toNat_add_toNat
+        (by simp only [BitVec.toNat_ofNat, Nat.reducePow, Nat.reduceMod]; omega)]
+      simp only [BitVec.toNat_ofNat, Nat.reducePow, Nat.reduceMod, ge_iff_le]; omega
+    · rw [BitVec.toNat_add_eq_toNat_add_toNat
+        (by simp only [BitVec.toNat_ofNat, Nat.reducePow, Nat.reduceMod]; omega)]
+      simp only [BitVec.toNat_ofNat, Nat.reducePow, Nat.reduceMod]; omega
+
+theorem extractLsByte_zeroExtend_shiftLeft (data : BitVec ((n + 1) * 8)) (hi : i > 0):
+    (BitVec.zeroExtend (n * 8) (data >>> 8)).extractLsByte (i - 1) = data.extractLsByte i := by
+  rcases i with rfl | i
+  · simp at hi
+  · apply BitVec.eq_of_getLsb_eq
+    intros j
+    simp only [Nat.add_one_sub_one, BitVec.getLsb_extractLsByte, BitVec.getLsb_zeroExtend,
+      BitVec.getLsb_ushiftRight]
+    by_cases hj : (j : Nat) ≤ 7
+    · simp only [hj, decide_True, Bool.true_and]
+      by_cases hi' : i * 8 + ↑j < n * 8
+      · simp only [hi', decide_True, Bool.true_and]
+        simp only at hi' ⊢
+        congr 1
+        omega
+      · by_cases hi' : i * 8 + ↑j < n * 8
+        · simp only [hi', decide_True, Bool.true_and]
+          congr 1
+          rw [Nat.add_mul]
+          omega
+        · simp only [hi', decide_False, Bool.false_and, Bool.false_eq]
+          apply BitVec.getLsb_ge
+          rw [Nat.add_mul, Nat.add_mul]
+          omega
+    · simp only [hj, decide_False, Bool.false_and]
+
+/--
+The byte at location `ix` in memory, such that `base ≤ ix ≤ base + ix` will be the `ix - base` byte of `data`.
+-/
+theorem write_bytes_eq_extractLsByte {ix base : BitVec 64} {m : Memory}
+  (lo : ix.toNat ≥ base.toNat)
+  (hi : ix.toNat < base.toNat + n) (hnowrap : base.toNat + n ≤ 2^64) :
+    m.write_bytes n base data ix = data.extractLsByte (ix - base).toNat := by
+  induction n generalizing base m ix
+  case zero => omega
+  case succ n ih =>
+    simp only [write_bytes]
+    by_cases hix : ix.toNat = base.toNat
+    · obtain hix : ix = base := by
+        apply BitVec.eq_of_toNat_eq hix
+      subst hix
+      simp only [BitVec.sub_self, BitVec.toNat_ofNat, Nat.reducePow, Nat.zero_mod]
+      rcases n with rfl | n
+      · simp only [Nat.reduceAdd, Nat.reduceMul, write_bytes_zero]
+        rw [write_of_eq (ix := ix) rfl]
+        rfl
+      · rw [write_bytes_eq_of_le]
+        · simp only [write_of_eq rfl, BitVec.extractLsByte_def, Nat.reduceAdd, Nat.reduceMul,
+            Nat.add_one_sub_one, Nat.sub_zero, BitVec.cast_eq]
+        · rw [BitVec.toNat_add_eq_toNat_add_toNat]
+          · simp only [BitVec.toNat_ofNat, Nat.reducePow, Nat.reduceMod, Nat.lt_add_one]
+          · simp only [BitVec.toNat_ofNat, Nat.reducePow, Nat.reduceMod]; omega
+        · rw [BitVec.toNat_add_eq_toNat_add_toNat
+            (by simp only [BitVec.toNat_ofNat, Nat.reducePow, Nat.reduceMod]; omega)]
+          simp only [BitVec.toNat_ofNat, Nat.reducePow, Nat.reduceMod]; omega
+    · rw [ih]
+      -- | TODO: make these into some kind of proof automation.
+      · have h_base_plus_1 : (base + 1#64).toNat = base.toNat + 1 := by
+          simp only [BitVec.toNat_add, BitVec.toNat_ofNat, Nat.reducePow, Nat.reduceMod]
+          rw [Nat.mod_eq_of_lt (by omega)]
+        have h_ix_sub_base_plus_1 : (ix - (base + 1#64)).toNat = ix.toNat - (base + 1#64).toNat := by
+          rw [BitVec.toNat_sub_eq_toNat_sub_toNat_of_le]
+          simp only [BitVec.le_def, BitVec.toNat_add, BitVec.toNat_ofNat, Nat.reducePow,
+            Nat.reduceMod]; omega
+        have h_ix_sub_base : (ix - base).toNat = ix.toNat - base.toNat := by
+          rw [BitVec.toNat_sub_eq_toNat_sub_toNat_of_le]
+          rw [BitVec.le_def]
+          omega
+        rw [h_ix_sub_base_plus_1, h_base_plus_1, h_ix_sub_base, Nat.sub_add_eq,
+          show ix.toNat - base.toNat - 1 = (ix.toNat - base.toNat) - 1 by omega]
+        apply extractLsByte_zeroExtend_shiftLeft
+        omega
+      · rw [BitVec.toNat_add_eq_toNat_add_toNat
+          (by simp only [BitVec.toNat_ofNat, Nat.reducePow, Nat.reduceMod]; omega)]
+        simp only [BitVec.toNat_ofNat, Nat.reducePow, Nat.reduceMod, ge_iff_le]; omega
+      · rw [BitVec.toNat_add_eq_toNat_add_toNat
+          (by simp only [BitVec.toNat_ofNat, Nat.reducePow, Nat.reduceMod]; omega)]
+        simp only [BitVec.toNat_ofNat, Nat.reducePow, Nat.reduceMod]; omega
+      · rw [BitVec.toNat_add_eq_toNat_add_toNat
+          (by simp only [BitVec.toNat_ofNat, Nat.reducePow, Nat.reduceMod]; omega)]
+        simp only [BitVec.toNat_ofNat, Nat.reducePow, Nat.reduceMod]; omega
+
+/--
+This is a low level theorem.
+Prefer using theorems from `Arm.Separate` that provide higher level theorems
+in terms of memory (non)-interference.
+-/
+theorem write_bytes_eq {mem : Memory} (hoverflow : base.toNat + n ≤ 2 ^ 64) :
+  ((write_bytes n base data mem) ix) =
+    if ix < base
+    then mem ix
+    else if ix.toNat ≥ base.toNat + n then mem ix
+    else data.extractLsByte (ix - base).toNat := by
+  by_cases h : ix < base
+  · simp only [h, ↓reduceIte]
+    apply write_bytes_eq_of_le h hoverflow
+  · simp only [h, ↓reduceIte]
+    by_cases h₂ : ix.toNat ≥ base.toNat + n
+    · simp only [ge_iff_le, h₂, ↓reduceIte]
+      apply write_bytes_eq_of_ge h₂ hoverflow
+    · simp only [ge_iff_le, h₂, ↓reduceIte]
+      apply write_bytes_eq_extractLsByte
+      · simp only [BitVec.not_lt] at h
+        rw [BitVec.le_def] at h
+        omega
+      · omega
+      · omega
+
+/--
+This is a low level theorem.
+Prefer using theorems from `Arm.Separate` that provide higher level theorems
+in terms of memory (non)-interference.
+-/
+theorem getLsb_write_bytes (hoverflow : base.toNat + n ≤ 2 ^ 64) :
+  ((write_bytes n base data mem) ix).getLsb i =
+  if ix < base
+  then (mem ix).getLsb i
+  else if ix.toNat ≥ base.toNat + n then (mem ix).getLsb i
+  else (data.extractLsByte (ix - base).toNat).getLsb i := by
+rw [write_bytes_eq hoverflow]
+by_cases h : ix < base
+· simp only [h, ↓reduceIte]
+· simp only [h, ↓reduceIte, ge_iff_le, BitVec.toNat_sub, Nat.reducePow, BitVec.getLsb_extractLsByte]
+  by_cases h₂ : base.toNat + n ≤ ix.toNat
+  · simp only [h₂, ↓reduceIte]
+  · simp only [h₂, ↓reduceIte, BitVec.getLsb_extractLsByte]
 
 end Memory
